eBPF-spec/types.dfy
@@ -1,128 +1,71 @@
-type int64 = x: int | -0x8000_0000_0000_0000 <= x < 0x8000_0000_0000_0000
-type uint64 = x: int | 0 <= x <= 0xFFFF_FFFF_FFFF_FFFF 
+module DataTypes {
 
-datatype Option<T> = None | Some(value: T)
-datatype CTXPermission = ReadOnly | ReadWrite | NoAccess
+    datatype ETYPEV =
+    | Uninit
+    | Scalar(kind: Kinds, val: bv64)
+    | PtrType(r: MemRegion, memid: nat, off: bv64)
+    | PtrOrNullType(r: MemRegion, memid: nat, off: bv64)
 
-datatype SIZE =
-    | B
-    | H
-    | W
-    | DW
-
-datatype SIGNNESS =
-    | SIGN
-    | UNSI
-
-datatype REGTYPE = 
-    | UNINT
-    | NULL
-    | SCALAR
-    //
-    | CTXMEM
-    | STACKMEM
-    //
-    | MAP_PTR
+    datatype MemRegion =
+    | PTR_TO_STACK
     | PTR_TO_MAP_VALUE
     | PTR_TO_MAP_KEY
-    //
     | PTR_TO_PACKET_META
-    | PTR_TO_PACKET
+    | PTR_TO_PACKET_DATA
     | PTR_TO_PACKET_END
-    //
     | PTR_TO_FLOW_KEYS
-    //
     | PTR_TO_SOCKET
-    | PTR_TO_SOCK_COMMON // TODO: what is the difference between PTR_TO_SOCKET and PTR_TO_SOCK_COMMON
+    | PTR_TO_SOCK_COMMON
     | PTR_TO_TCP_SOCK
     | PTR_TO_XDP_SOCK
-    //
     | PTR_TO_TP_BUFFER
-    //
-    | PTR_TO_ARENA
-    //
-    | PTR_TO_FUNC
-    //
-    | STACK_ITER
-    | STACK_DYNPTR
+    | PTR_TO_BUF
+    | PTR_TO_MEM
+    | PTR_TO_MAP_META
+    | PTR_TO_CTX
+    | PTR_TO_BTF
+    // | PTR_TO_ARENA
+    // | PTR_TO_FUNC
 
-    /*
-    NOT_INIT = 0,        /* nothing was written into register */
-    SCALAR_VALUE,        /* reg doesn't contain a valid pointer */
-    PTR_TO_CTX,      /* reg points to bpf_context */
-    CONST_PTR_TO_MAP,    /* reg points to struct bpf_map */
-    PTR_TO_MAP_VALUE,    /* reg points to map element value */
-    PTR_TO_STACK,        /* reg == frame_pointer + offset */
+    function r2id(r: MemRegion): (res: nat)
+    {
+        match r
+            case PTR_TO_STACK       => 0
+            case PTR_TO_MAP_VALUE   => 1
+            case PTR_TO_MAP_KEY     => 2
+            case PTR_TO_PACKET_META => 3
+            case PTR_TO_PACKET_DATA => 4
+            case PTR_TO_PACKET_END  => 5
+            case PTR_TO_FLOW_KEYS   => 6
+            case PTR_TO_SOCKET      => 7
+            case PTR_TO_SOCK_COMMON => 8
+            case PTR_TO_TCP_SOCK    => 9
+            case PTR_TO_XDP_SOCK    => 10
+            case PTR_TO_TP_BUFFER   => 11
+            case PTR_TO_BUF         => 12
+            case PTR_TO_MEM         => 13
+            case PTR_TO_MAP_META    => 14
+            case PTR_TO_CTX         => 15
+            case PTR_TO_BTF         => 16
+    }
 
-    PTR_TO_PACKET_META,  /* skb->data - meta_len */
-    PTR_TO_PACKET_END,   /* skb->data + headlen */
-    PTR_TO_PACKET,       /* reg points to skb->data */
+    datatype Kinds =
+    | Normal
+    | SpecialPtr
+    // | Iter
+    // | Dynptr
 
-    PTR_TO_FLOW_KEYS,    /* reg points to bpf_flow_keys */
+    datatype MEMTYPE =
+    | GENERAL
+    | RAW
+    | STRUCT
 
-    PTR_TO_SOCKET,       /* reg points to struct bpf_sock */
-    PTR_TO_SOCK_COMMON,  /* reg points to sock_common */
-    PTR_TO_TCP_SOCK,     /* reg points to struct tcp_sock */
-    PTR_TO_XDP_SOCK,     /* reg points to struct xdp_sock */
+    datatype ACCESSPERM =
+    | NOACCESS
+    | READONLY
+    | RDWR
 
-        CONST_PTR_TO_DYNPTR,     /* reg points to a const struct bpf_dynptr */
-
-    // LOCK
-
-    PTR_TO_MAP_KEY,      /* reg points to a map element key */
-
-    PTR_TO_TP_BUFFER,    /* reg points to a writable raw tp's buffer */
-        PTR_TO_BTF_ID,
-
-
-        PTR_TO_MEM,      /* reg points to valid memory region */
-    PTR_TO_ARENA,
-        PTR_TO_BUF,      /* reg points to a read/write buffer */
-    PTR_TO_FUNC,         /* reg points to a bpf program function */
-    */
-
-datatype REG = 
-    | R0
-    | R1
-    | R2
-    | R3
-    | R4
-    | R5
-    | R6
-    | R7
-    | R8
-    | R9
-    | R10
-    | Rn
-
-datatype ATOMICOP =
-    | ATOMIC_ADD
-    | ATOMIC_AND
-    | ATOMIC_OR
-    | ATOMIC_XOR
-    | ATOMIC_FETCH_ADD
-    | ATOMIC_FETCH_AND
-    | ATOMIC_FETCH_OR
-    | ATOMIC_FETCH_XOR
-    | ATOMIC_XCHG
-    | ATOMIC_CMPXCHG
-
-// Less or greater jump
-datatype LGJMP =
-    | JGT
-    | JGE
-    | JSGT
-    | JSGE
-    | JLT
-    | JLE
-    | JSLT
-    | JSLE
-
-datatype ACCESSTYPE =
-    | READ
-    | WRITE
-
-datatype ProgTypes =
+    datatype ProgTypes =
     | BPF_PROG_TYPE_SOCKET_FILTER
     | BPF_PROG_TYPE_SCHED_CLS
     | BPF_PROG_TYPE_SCHED_ACT
@@ -156,7 +99,7 @@ datatype ProgTypes =
     | BPF_PROG_TYPE_SYSCALL
     | BPF_PROG_TYPE_NETFILTER
 
-datatype AttachTypes =
+    datatype AttachTypes =
     | BPF_CGROUP_INET_INGRESS
     | BPF_CGROUP_INET_EGRESS
     | BPF_CGROUP_INET_SOCK_CREATE
@@ -164,7 +107,7 @@ datatype AttachTypes =
     | BPF_SK_SKB_STREAM_PARSER
     | BPF_SK_SKB_STREAM_VERDICT
     | BPF_CGROUP_DEVICE
-    | BPF_SK_MSG_VERDICT
+    | BPF_SK_MSG_VERDICT    
     | BPF_CGROUP_INET4_BIND
     | BPF_CGROUP_INET6_BIND
     | BPF_CGROUP_INET4_CONNECT
@@ -214,7 +157,7 @@ datatype AttachTypes =
     | BPF_NETKIT_PRIMARY
     | BPF_NETKIT_PEER
 
-datatype MapTypes =
+    datatype MapTypes =
     | BPF_MAP_TYPE_HASH
     | BPF_MAP_TYPE_ARRAY
     | BPF_MAP_TYPE_PROG_ARRAY
@@ -251,46 +194,7 @@ datatype MapTypes =
     | BPF_MAP_TYPE_CGRP_STORAGE
     | BPF_MAP_TYPE_ARENA
 
-class RegState {
-    ghost var regNo: REG
-    ghost var regType: REGTYPE
-    ghost var regVal: bv64
-    ghost var mapFd: int64
-    ghost var memId: int64
-
-    ghost constructor {:axiom} (regNo: REG)
-        ensures this.regNo == regNo
-        ensures this.regVal == 0
-        ensures this.regType == UNINT
-        // Cannot combine mapFd and memId together as for PTR_TO_MAP_VALUE,
-        // we need to know the memId for multiple lookups and its mapFd to know which map
-        ensures this.mapFd == -1
-        /*
-            Stack: frameNo
-            CONST_PTR_TO_MAP: different maps
-            PTR_TO_MAP_VALUE: different returned memory
-            ...
-        */
-        ensures this.memId == -1
-}
-
-class MapState {
-    ghost var mapType: MapTypes
-    ghost var keySize: int64
-    ghost var valSize: int64
-    ghost var maxEntries: int64
-    ghost var mapFlag: int64        // TODO: remove?
-    ghost var readable: bool
-    ghost var writable: bool
-    ghost var innerMapFd: int64
-}
-
-class SpinLockState{
-    ghost var isLocked: bool
-    ghost var memId:    int64
-    ghost var ptrType:  REGTYPE
-}
-
-class MutableVars{
-    ghost var idCounter: int64
+    type int64 = x: int | -0x8000_0000_0000_0000 <= x < 0x8000_0000_0000_0000
+    
+    type s16 = x: int | -0x8000 <= x < 0x8000
 }
