eBPF-spec/utils.dfy
@@ -1,108 +1,144 @@
 include "types.dfy"
-include "ctxmem-precond.dfy"
+include "terms.dfy"
+include "states.dfy"
 
-function signExtend32To64(num: bv64) :bv64
-    {
-        signExtend64(num, 32)
-    }
+module Utils {
 
-function signExtend64(num: bv64, curwidth: int) :bv64
-    requires curwidth == 8 || curwidth == 16 || curwidth == 32 || curwidth == 64
-    {
-        if curwidth == 64 then num
-        else if curwidth == 32 then (
-            if num & 0x0000_0000_8000_0000 == 0
-                then (num & 0x0000_0000_FFFF_FFFF)
-            else (num | 0xFFFF_FFFF_0000_0000)
+    import opened Terms
+    import opened DataTypes
+    import opened States
+
+
+    // ----------------- safety properties ---------------------
+
+    ghost predicate sp4_vm_integrity(dst: REG) {dst != R10}
+
+    ghost predicate sp2_datasafe(s: State, reg: REG)
+    {   
+        var regtv := get_reg_typeval(s, reg);
+        regtv != Uninit && (
+            if !s.cfg.allow_ptr_leak
+            then is_scalar(regtv)
+            else true
         )
-        else if curwidth == 16 then (
-            if num & 0x0000_0000_0000_8000 == 0
-                then (num & 0x0000_0000_0000_FFFF)
-            else (num | 0xFFFF_FFFF_FFFF_0000)
-        )
-        // curwidth == 8 
-        else (
-            if num & 0x0000_0000_0000_0080 == 0
-                then (num & 0x0000_0000_0000_00FF)
-            else (num | 0xFFFF_FFFF_FFFF_FF00)
-        )
-        // else if num & (0x1 << ((curwidth-1) as bv6)) == 0 then (num & 0x0000_0000_FFFF_FFFF)
-        // else num | !(((0x1 as bv64) << (curwidth as bv6)) - 0x1)
+    }
+
+    // -----------   reg type and value check retrival -------------
+
+    ghost function get_reg_typeval(s: State, reg: REG): ETYPEV
+        {
+            match reg {
+                case R0 => s.R0
+                case R1 => s.R1
+                case R2 => s.R2
+                case R3 => s.R3
+                case R4 => s.R4
+                case R5 => s.R5
+                case R6 => s.R6
+                case R7 => s.R7
+                case R8 => s.R8
+                case R9 => s.R9
+                case R10 => s.R10
+                // case Rn => s.Rn
+            }
+        }
+
+    function is_scalar(e: ETYPEV): bool {
+        match e
+        case Scalar(_, _) => true
+        case _           => false
     }
 
 
-// Flip bits and then add 1, finally remove the sign bit
-function twocom2Abs32Bit(num: bv64) :bv64
+    function is_scalar_zero(e: ETYPEV): bool {
+        match e
+        case Scalar(_, 0) => true
+        case _           => false
+    }
+
+    function ptr_or_ptrornull(e: ETYPEV): bool {
+        match e
+        case PtrOrNullType(_, _, _)   => true
+        case PtrType(_, _, _)         => true
+        case _                  => false
+    }
+
+    function ptrornull(e: ETYPEV): bool {
+        match e
+        case PtrOrNullType(_, _, _)   => true
+        case _                  => false
+    }
+
+    function is_ptr(e: ETYPEV): bool {
+        match e
+        case PtrType(_, _, _)         => true
+        case _                  => false
+    }
+
+    function ptrnull_to_ptr(e: ETYPEV) : (res: ETYPEV)
+        requires ptrornull(e)
+        ensures is_ptr(res)
     {
-        if num & 0x80000000 == 0 then num & 0xEFFF_FFFF
-        else ((!num) + 1) & 0xEFFF_FFFF
+        match e
+        case PtrOrNullType(t, memid, off) => ETYPEV.PtrType(t, memid, off)
+        case _ => e
     }
 
-// Flip bits and then add 1, finally remove the sign bit
-function twocom2Abs64Bit(num: bv64) :bv64
+    // ------------------- reg state reconstruction -------------------
+
+    ghost function new_state_regonly(
+        s: State, reg: REG, reg_state: ETYPEV
+    ): (res: State)
+    //
+    requires reg != R10
+    ensures s.R10 == res.R10
+    ensures s.mems == res.mems
+    ensures forall r | r != reg
+            :: get_reg_typeval(s, r) == get_reg_typeval(res, r)
+    ensures get_reg_typeval(res, reg) == reg_state
     {
-        if num & 0x8000000000000000 == 0 then num
-        else ((!num) + 1) & 0x7FFF_FFFF_FFFF_FFFF
+      match reg
+        case R0 =>  s.(R0  := reg_state)
+        case R1 =>  s.(R1  := reg_state)
+        case R2 =>  s.(R2  := reg_state)
+        case R3 =>  s.(R3  := reg_state)
+        case R4 =>  s.(R4  := reg_state)
+        case R5 =>  s.(R5  := reg_state)
+        case R6 =>  s.(R6  := reg_state)
+        case R7 =>  s.(R7  := reg_state)
+        case R8 =>  s.(R8  := reg_state)
+        case R9 =>  s.(R9  := reg_state)
+        case R10 => s.(R10 := reg_state)
+        // case Rn =>  s.(Rn  := reg_state)
     }
+    
+    // --------------------arith operation helpers -------------------------
 
-function abs2NegTwocom32Bit(num: bv64) :bv64
-    {
-        (((!num) + 1) & 0xFFFFFFFF) | 0x8000_0000
-    }
-
-function abs2NegTwocom64Bit(num: bv64) :bv64
-    {
-        ((!num) + 1) | 0x8000_0000_0000_0000
-    }
-
-function bv64ToInt64(num: bv64) :int64
-    {
-        if num & 0x8000_0000_0000_0000 == 0 then (num as int64)
-        else -(twocom2Abs64Bit(num) as int64)
-    }
-
-function bv64ToUInt64(num: bv64) :uint64
-    {
-        (num as uint64)
-    }
-
-function bv32ToInt32(num: bv64) :int64
-    // requires num & 0xFFFF_FFFF_0000_0000 == 0
-    {
-        if num & 0x8000_0000 == 0 then ((num & 0x0000_0000_FFFF_FFFF) as int64)
-        else -(twocom2Abs32Bit(num) as int64)
-    }
-
-// truncate
-
-function bv64Tobv32(num: bv64) :bv64
-    {
-        num & 0x0000_0000_FFFF_FFFF
-    }
-
-// Byte swap
-
-function {:fuel 8} byteswapN(num: bv64, curb: int, N: int) :bv64
-    requires 0 <= curb < 8
-    requires N == 2 || N == 4 || N == 8
-    requires curb < N
-    decreases 8-curb
-    {
-        if curb+1 ==  N then (((num >> (curb * 8)) & 0xff) << ((N-curb-1) * 8))
-        else ((((num >> (curb * 8)) & 0xff) << ((N-curb-1) * 8)) | (byteswapN(num, curb+1, N)))
-    }
-
-
-// Signed division
-
-function signDiv32Bit(dividend: bv64, divisor: bv64) :bv64
+    ghost function bvadd64(x: bv64, y: bv64): bv64 { x + y }
+    ghost function bvadd32(x: bv64, y: bv64): bv64 { low32(x + y) }
+    //
+    ghost function bvsub64(x: bv64, y: bv64): bv64 { x - y }
+    ghost function bvsub32(x: bv64, y: bv64): bv64 { low32(x - y) }
+    //
+    ghost function bvmul64(x: bv64, y: bv64): bv64 { x * y }
+    ghost function bvmul32(x: bv64, y: bv64): bv64 { low32(x * y) }
+    
+    ghost function bvdiv64(x: bv64, y: bv64): bv64 
+    requires y != 0
+    { x / y }
+    
+    ghost function bvdiv32(x: bv64, y: bv64): bv64
+    requires low32(y) != 0
+    { low32(low32(x) / low32(y)) }
+    
+    function bvsdiv32(dividend: bv64, divisor: bv64) :bv64
     requires twocom2Abs32Bit(divisor) != 0x0
     {
         if (dividend & 0x80000000) == (divisor & 0x80000000) then (twocom2Abs32Bit(dividend) / twocom2Abs32Bit(divisor))
         else abs2NegTwocom32Bit((twocom2Abs32Bit(dividend) / twocom2Abs32Bit(divisor)))
     }
-
-function signDiv64Bit(dividend: bv64, divisor: bv64) :bv64
+    
+    function bvsdiv64(dividend: bv64, divisor: bv64) :bv64
     requires twocom2Abs64Bit(divisor) != 0x0
     {
         if (dividend & 0x8000000000000000) == (divisor & 0x8000000000000000)
@@ -110,293 +146,1166 @@ function signDiv64Bit(dividend: bv64, divisor: bv64) :bv64
             // Convert dividend and divisor to absolute value and then calculate and then negate the result
             else abs2NegTwocom64Bit(twocom2Abs64Bit(dividend) / twocom2Abs64Bit(divisor))
     }
-
-
-/*
-function signMod32Bit(dividend: bv64, divisor: bv64) :bv64
-    requires twocom2Abs32Bit(divisor) != 0x0
-    {
-        if (dividend & 0x80000000) == (divisor & 0x80000000)
-            then (twocom2Abs32Bit(dividend) % twocom2Abs32Bit(divisor))
-            else abs2NegTwocom32Bit(twocom2Abs32Bit(dividend) % twocom2Abs32Bit(divisor))
-    }
-
-function signMod64Bit(dividend: bv64, divisor: bv64) :bv64
-    requires twocom2Abs64Bit(divisor) != 0x0
-    {
-        if (dividend & 0x8000000000000000) == (divisor & 0x8000000000000000)
-            then (twocom2Abs64Bit(dividend) % twocom2Abs64Bit(divisor))
-            else abs2NegTwocom64Bit(twocom2Abs64Bit(dividend) % twocom2Abs64Bit(divisor))
-    }
-*/
-
-// Signed modulo: a % n = a - n * trunc(a / n)
-
-function signMod32Bit(dividend: bv64, divisor: bv64) :bv64
-    requires twocom2Abs32Bit(divisor) != 0x0
-    {
-        (dividend - (divisor * signDiv32Bit(dividend, divisor))) & 0x0000_0000_FFFF_FFFF
-    }
-
-function signMod64Bit(dividend: bv64, divisor: bv64) :bv64
+    
+    ghost function bvmod64(x: bv64, y: bv64): bv64
+    requires y != 0
+    { x % y }
+    
+    ghost function bvmod32(x: bv64, y: bv64): bv64
+    requires low32(y) != 0
+    { low32(low32(x) % low32(y)) }
+    
+    // Signed modulo: a % n = a - n * trunc(a / n)
+    function bvsmod64(dividend: bv64, divisor: bv64) :bv64
     requires twocom2Abs64Bit(divisor) != 0
     {
-        dividend - (divisor * signDiv64Bit(dividend, divisor))
+        dividend - (divisor * bvsdiv64(dividend, divisor))
     }
 
+    function bvsmod32(dividend: bv64, divisor: bv64) :bv64
+    requires twocom2Abs32Bit(divisor) != 0x0
+    {
+        (dividend - (divisor * bvsdiv32(dividend, divisor))) & 0x0000_0000_FFFF_FFFF
+    }
 
-// Airthmetic right shift
+    ghost function bvnot64(x: bv64): bv64 { !x }
+    ghost function bvnot32(x: bv64): bv64 { low32(!x) }
 
-function signShift32Bit(num: bv64, shift: bv64) :bv64
+    ghost function bvor64(x: bv64, y: bv64): bv64 { x | y }
+    ghost function bvor32(x: bv64, y: bv64): bv64 { low32(x | y) }
+
+    ghost function bvand64(x: bv64, y: bv64): bv64 { x & y }
+    ghost function bvand32(x: bv64, y: bv64): bv64 { low32(x & y) }
+
+    ghost function bvxor64(x: bv64, y: bv64): bv64 { x ^ y }
+    ghost function bvxor32(x: bv64, y: bv64): bv64 { low32(x ^ y) }
+
+
+    ghost function bvlshr32(num: bv64, shift: bv64) : bv64
+    {num >> ((shift & 0x1F) as bv5)}
+
+    ghost function bvlshr64(num: bv64, shift: bv64) : bv64
+    {num >> ((shift & 0x3F) as bv6)}
+
+    function bvashr32(num: bv64, shift: bv64) :bv64
     {
         if (num & 0x80000000 == 0) then (num >> ((shift & 0x1F) as bv5)) & 0xFFFFFFFF
         else ((num >> ((shift & 0x1F) as bv5)) | !(((0x1 as bv64) << ((32-(shift & 0x1F)) as bv8)) - 0x1)) & 0xFFFFFFFF
     }
 
-function signShift64Bit(num: bv64, shift: bv64) :bv64
+    function bvashr64(num: bv64, shift: bv64) :bv64
     {
         if (num & 0x8000000000000000) == 0 then (num >> ((shift & 0x3F) as bv6))
         else ((num >> ((shift & 0x3F) as bv6)) | !(((0x1 as bv64) << ((64-(shift & 0x3F)) as bv8)) - 0x1))
     }
 
-// Memory related functions
+    ghost function bvshl32(num: bv64, shift: bv64) : bv64
+    {num << ((shift & 0x1F) as bv5)}
 
-function getRegByteX(num: bv64, byteIdx:int) :bv8
-    requires 0 <= byteIdx < 8
+    ghost function bvshl64(num: bv64, shift: bv64) : bv64
+    {num << ((shift & 0x3F) as bv6)}
+
+    // ----
+
+    ghost predicate unknown_bool()
+
+    ghost predicate bv_eq(x: bv64, y: bv64) {x == y}
+
+    ghost predicate bv_neq(x: bv64, y: bv64) {x != y}
+
+    ghost predicate is_32bit_zero(x: bv64) {low32(x) == 0}
+
+    ghost predicate not_32bit_zero(x: bv64) {low32(x) != 0}
+    
+    ghost predicate is_64bit_zero(x: bv64) {x == 0}
+
+    ghost predicate not_64bit_zero(x: bv64) {x != 0}
+
+    ghost predicate bit8signed(val: bv64) {(val & 0x0000000000000080) != 0 }
+
+    ghost predicate bit16signed(val: bv64) {(val & 0x0000000000008000) != 0 }
+
+    ghost predicate bit32signed(val: bv64) {(val & 0x0000000080000000) != 0 }
+
+    function low32(val: bv64) : bv64 {val & 0x0000_0000_FFFF_FFFF}
+    
+    ghost function low16(val: bv64) : bv64 {val & 0x0000_0000_0000_FFFF}
+
+    ghost function low8(val: bv64) : bv64 {val & 0x0000_0000_0000_00FF}
+
+    ghost function low5(val: bv64) : bv64 {val & 0x0000_0000_0000_001F}
+
+    ghost function low6(val: bv64) : bv64 {val & 0x0000_0000_0000_003F}
+
+    function bv64ToInt64(num: bv64) :int64
     {
-        ((num >> (byteIdx*8)) & 0xff) as bv8
+        if num & 0x8000_0000_0000_0000 == 0 then (num as int64)
+        else -(twocom2Abs64Bit(num) as int64)
     }
 
-// When loading, not necessary to use old() expression as we are not modifying anything with `modifies`
-// NOTE: cannot call this function, if there is modifies on this mem
-/*
-ghost function loadNbytesStack(mem: array<bv8>, memLen: int64, off: int64, idx:int64, size: int64) :bv64
-    reads mem
-    requires mem.Length == memLen
-    requires size == 1 || size == 2 || size == 4 || size == 8
-    requires 0<= idx < size
-    requires 0 <= off + idx < off+size <= memLen
-    decreases size-idx
-    ensures size == 4 ==> loadNbytesStack(mem, memLen, off, idx, size) & 0xFFFF_FFFF_0000_0000 == 0x0
-    ensures size == 2 ==> loadNbytesStack(mem, memLen, off, idx, size) & 0xFFFF_FFFF_FFFF_0000 == 0x0
-    ensures size == 1 ==> loadNbytesStack(mem, memLen, off, idx, size) & 0xFFFF_FFFF_FFFF_FF00 == 0x0
+    function bv32ToInt32(num: bv64) :int64
     {
-        var curByte := ((mem[off+idx] as bv64) << ((idx * 8) as bv6));
-        if idx+1 == size then curByte
-        else curByte | loadNbytesStack(mem, memLen, off, idx+1, size)
+        if num & 0x8000_0000 == 0 then ((num & 0x0000_0000_FFFF_FFFF) as int64)
+        else -(twocom2Abs32Bit(num) as int64)
     }
-*/
 
-ghost function loadNbytesMem(mem: array<bv8>, off: int64, size: int64) :bv64
-    reads mem
-    requires size == 1 || size == 2 || size == 4 || size == 8
-    requires 0 <= off < off+size <= mem.Length
+    // Flip bits and then add 1, finally remove the sign bit
+    function twocom2Abs64Bit(num: bv64) :bv64
+    {
+        if num & 0x8000000000000000 == 0 then num
+        else ((!num) + 1) & 0x7FFF_FFFF_FFFF_FFFF
+    }
+
+    // Flip bits and then add 1, finally remove the sign bit
+    function twocom2Abs32Bit(num: bv64) :bv64
+    {
+        if num & 0x80000000 == 0 then num & 0xEFFF_FFFF
+        else ((!num) + 1) & 0xEFFF_FFFF
+    }
+
+    function abs2NegTwocom32Bit(num: bv64) :bv64
+        {
+            (((!num) + 1) & 0xFFFFFFFF) | 0x8000_0000
+        }
+
+    function abs2NegTwocom64Bit(num: bv64) :bv64
+        {
+            ((!num) + 1) | 0x8000_0000_0000_0000
+        }
+
+    function {:fuel 8} nbytes_wap(num: bv64, N: int) :bv64
+    requires N == 2 || N == 4 || N == 8
+    {
+        byteswap_iter(num, 0, N)
+    }
+
+    function {:fuel 8} byteswap_iter(num: bv64, curb: int, N: int) :bv64
+    requires 0 <= curb < 8
+    requires N == 2 || N == 4 || N == 8
+    requires curb < N
+    decreases 8-curb
+    {
+        if curb+1 ==  N then (((num >> (curb * 8)) & 0xff) << ((N-curb-1) * 8))
+        else ((((num >> (curb * 8)) & 0xff) << ((N-curb-1) * 8)) | (byteswap_iter(num, curb+1, N)))
+    }
+
+    function signext_bits_n2m_low_perf(num:bv64, n: nat, m: nat) : bv64
+    requires (n, m) == (8, 32) || (n, m) == (16, 32) ||
+             (n, m) == (8, 64) || (n, m) == (16, 64) ||
+             (n, m) == (32, 64)
+    {
+        var sign_bit := (1 << (n-1));
+        var bit_n_mask := ((1 << n) -1);
+        var ext_sign_bits := 
+                !bit_n_mask &
+                if m == 32
+                then 0x0000_0000_FFFF_FFFF
+                else 0xFFFF_FFFF_FFFF_FFFF
+                ;
+
+        if (num & sign_bit) != 0
+        then (bit_n_mask & num) | ext_sign_bits
+        else bit_n_mask & num
+    }
+    
+    ghost function signext_bits_n2m(num:bv64, n: nat, m: nat) : bv64
+    requires (n, m) == (8, 32) || (n, m) == (16, 32) ||
+             (n, m) == (8, 64) || (n, m) == (16, 64) || (n, m) == (32, 64)
+    ensures signext_bits_n2m(num, n, m) == signext_bits_n2m_low_perf(num, n, m)
+    {
+        match (n, m) {
+            case (8, 32) =>
+                if bit8signed(num)
+                then bvor32(num, 0x00000000FFFFFF00)
+                else low8(num)
+
+            case (16, 32) =>
+                if bit16signed(num)
+                then bvor32(num, 0x00000000FFFF0000)
+                else low16(num)
+
+            case (8, 64) =>
+                if bit8signed(num)
+                then bvor64(num, 0xFFFFFFFFFFFFFF00)
+                else low8(num)
+
+            case (16, 64) =>
+                if bit16signed(num)
+                then bvor64(num, 0xFFFFFFFFFFFF0000)
+                else low16(num)
+
+            case (32, 64) =>
+                if bit32signed(num)
+                then bvor64(num, 0xFFFFFFFF00000000)
+                else low32(num)
+        }
+    }
+
+    lemma signext_two_impls_equal(num:bv64, n: nat, m: nat)
+    requires (n, m) == (8, 32) || (n, m) == (16, 32) ||
+             (n, m) == (8, 64) || (n, m) == (16, 64) ||
+             (n, m) == (32, 64)
+    ensures signext_bits_n2m(num, n, m) == signext_bits_n2m_low_perf(num, n, m)
+    {}
+
+    ghost function signext_byte_nto8(num:bv64, size: SIZE) : (res: bv64)
+    ensures forall i | 0 <= i < size_to_nat(size)
+            :: get_nth_byte(res, i) == get_nth_byte(res, i)
+    {
+        match size {
+            case B  => signext_bits_n2m(num, 8, 64)
+            case HW => signext_bits_n2m(num, 16, 64)
+            case W  => signext_bits_n2m(num, 32, 64)
+            case _  => num
+        }
+    }
+
+    ghost function get_reg_arith_val(s: State, reg: REG) : (res: bv64)
+    requires get_reg_typeval(s, reg) != Uninit
+    requires valid_etypev_if_ptr(s, get_reg_typeval(s, reg))
+    ensures var tv := get_reg_typeval(s, reg);
+            is_scalar(tv) ==> (res == tv.val)
+    {
+        var regtv := get_reg_typeval(s, reg);
+        get_arith_val(s, regtv)
+    }
+
+
+    ghost function get_arith_val(s: State, regtv: ETYPEV) : (res: bv64)
+    requires regtv != Uninit
+    requires valid_etypev_if_ptr(s, regtv)
+    ensures is_scalar(regtv) ==> (res == regtv.val)
+    {
+        match regtv {
+
+            case Scalar(_, val)             => val
+
+            case PtrType(r1, memid1, off1)  => 
+                bvadd64(s.mems[r2id(r1)][memid1].base, off1)
+
+            case PtrOrNullType(r2, memid2, off2) => (
+                var unknown: bool :| true;
+                if unknown
+                then bvadd64(s.mems[r2id(r2)][memid2].base, off2)
+                else 0
+            )
+            case _ => (
+                assert false;
+                -1
+            )
+        }
+    }
+
+    // ------------------------- Memory operation helpers ----------------
+
+
+    ghost function get_ptr_info(addr_tv: ETYPEV, ioff: s16) : (nat, nat, int)
+    requires is_ptr(addr_tv)
+    {
+        var rid := r2id(addr_tv.r);
+        var memid := addr_tv.memid;
+            
+        var cur_off := 
+            if addr_tv.r == PTR_TO_STACK
+            then bv64ToInt64(addr_tv.off) + ioff + 512
+            else bv64ToInt64(addr_tv.off) + ioff;
+        
+        (rid, memid, cur_off)
+    }
+
+    function size_to_nat(sz: SIZE) : nat
+    {
+        match sz {
+            case B   =>  1
+            case HW  =>  2
+            case W   =>  4
+            case DW  =>  8
+        }
+    }
+
+    ghost function get_nth_byte(num: bv64, byte_idx:int) : bv64
+    requires 0 <= byte_idx < 8
+    {
+        match byte_idx {
+
+            case 0 => num & 0xff
+
+            case 1 => (num >> 8) & 0xff
+
+            case 2 => (num >> 16) & 0xff
+
+            case 3 => (num >> 24) & 0xff
+
+            case 4 => (num >> 32) & 0xff
+
+            case 5 => (num >> 40) & 0xff
+
+            case 6 => (num >> 48) & 0xff
+
+            case 7 => (num >> 56) & 0xff
+
+            case _ => (
+                assert false;
+                0
+            )
+        }
+    }
+
+    ghost function low_nsize(val: bv64, size: SIZE) : bv64
+    {
+        match size {
+            case B  => low8(val)
+            case HW => low16(val)
+            case W  => low32(val)
+            case DW => val
+        }
+    }
+
+    ghost predicate same_type(tv1: ETYPEV, tv2: ETYPEV)
+    {
+        match (tv1, tv2) {
+            case (PtrOrNullType(_, _, _), PtrOrNullType(_, _, _)) => true
+            case (PtrType(_, _, _), PtrType(_, _, _)) => true
+            case (Scalar(_, _), Scalar(_, _)) => true
+            case (Uninit, Uninit) => true
+            case _ => false
+        }
+    }
+
+    predicate all_slots_scalars(slots: seq<MemSlot>)
+    {
+        forall i | 0 <= i < |slots|
+        ::
+        is_scalar(slots[i].etypev)
+    }
+
+    ghost function etypev_to_val(tv: ETYPEV) : bv64
+    requires tv != Uninit
+    {
+        match tv {
+            case Uninit => (
+                assert false;
+                -1
+            )
+            case Scalar(_, val) => val
+            case PtrType(_, _, off) => off
+            case PtrOrNullType(_, _, off) => off
+        }
+    }
+
+    ghost function read_8_byte_data(data: seq<MemSlot>, alg_off: int) : (res: bv64)
+    requires 0 <= alg_off < alg_off + 8 <= |data|
+    requires forall i | 0 <= alg_off <= i < alg_off + 8
+             ::
+             data[i].etypev != Uninit
+    {
+        ((etypev_to_val(data[alg_off + 0].etypev) & 0xff))        |
+        ((etypev_to_val(data[alg_off + 1].etypev) & 0xff) << 8)   |
+        ((etypev_to_val(data[alg_off + 2].etypev) & 0xff) << 16)  |
+        ((etypev_to_val(data[alg_off + 3].etypev) & 0xff) << 24)  |
+        ((etypev_to_val(data[alg_off + 4].etypev) & 0xff) << 32)  |
+        ((etypev_to_val(data[alg_off + 5].etypev) & 0xff) << 40)  |
+        ((etypev_to_val(data[alg_off + 6].etypev) & 0xff) << 48)  |
+        ((etypev_to_val(data[alg_off + 7].etypev) & 0xff) << 56)
+    }
+
+    ghost function {:timeLimit 20} read_n_byte_data(
+        data: seq<MemSlot>, cur_off: int, size: SIZE, sign_ext: bool
+    ) : (res: bv64)
+    requires 0 <= cur_off < cur_off + size_to_nat(size) <= |data|
+    requires forall i | cur_off <= i < cur_off + size_to_nat(size)
+             :: data[i].etypev != Uninit
+    {
+        match size {
+                
+            case B  =>
+                (etypev_to_val(data[cur_off+0].etypev) & 0xff)
+                
+            case HW =>
+                ((etypev_to_val(data[cur_off+0].etypev) & 0xff))        | 
+                ((etypev_to_val(data[cur_off+1].etypev) & 0xff) << 8)
+                
+            case W  =>
+                ((etypev_to_val(data[cur_off+0].etypev) & 0xff))        | 
+                ((etypev_to_val(data[cur_off+1].etypev) & 0xff) << 8)   |
+                ((etypev_to_val(data[cur_off+2].etypev) & 0xff) << 16)  | 
+                ((etypev_to_val(data[cur_off+3].etypev) & 0xff) << 24)
+                
+            case DW =>
+                ((etypev_to_val(data[cur_off].etypev) & 0xff))          |
+                ((etypev_to_val(data[cur_off+1].etypev) & 0xff) << 8)   |
+                ((etypev_to_val(data[cur_off+2].etypev) & 0xff) << 16)  | 
+                ((etypev_to_val(data[cur_off+3].etypev) & 0xff) << 24)  |
+                ((etypev_to_val(data[cur_off+4].etypev) & 0xff) << 32)  | 
+                ((etypev_to_val(data[cur_off+5].etypev) & 0xff) << 40)  |
+                ((etypev_to_val(data[cur_off+6].etypev) & 0xff) << 48)  | 
+                ((etypev_to_val(data[cur_off+7].etypev) & 0xff) << 56)
+        }
+    }
+
+    lemma read_n_byte_data_inv(data: seq<MemSlot>, cur_off: int, size: SIZE)
+    requires 0 <= cur_off < cur_off + size_to_nat(size) <= |data|
+    requires forall i | 0 <= cur_off <= i < cur_off + size_to_nat(size)
+                 ::
+                 data[i].etypev != Uninit
+    ensures forall i | 0 <= i < size_to_nat(size)
+             ::
+             get_nth_byte(read_n_byte_data(data, cur_off, size, false), i) == (
+                 etypev_to_val(data[cur_off+i].etypev) & 0xff
+             )
+    {}
+
+    ghost predicate slots_inited(
+        s: State, addr_tv: ETYPEV, ioff: s16, size: SIZE
+    )
+    requires is_ptr(addr_tv) && valid_etypev_if_ptr(s, addr_tv)
+    {
+        var (rid, memid, cur_off) := get_ptr_info(addr_tv, ioff);
+
+        var data := s.mems[rid][memid].data;
+
+        forall i | 0 <= cur_off <= i < cur_off + size_to_nat(size)
+             ::
+             i < |data|
+             &&
+             data[i].etypev != Uninit
+    }
+
+    ghost function {:timeLimit 3} read_n_byte_etypev(
+        s: State, addr_tv: ETYPEV,
+        ioff: s16, size: SIZE, sign_ext: bool
+    ) : (res: ETYPEV)
+    requires is_ptr(addr_tv) && valid_etypev_if_ptr(s, addr_tv)
+    requires addr_tv.r == PTR_TO_CTX && size == W ==> packet_mems_exist(s)
+    requires access_mem_slots_valid(s, addr_tv, ioff, size)
+    requires slots_inited(s, addr_tv, ioff, size)
     //
+    ensures valid_etypev_if_ptr(s, res)
     {
-        if (size == 1)
-            then (mem[off] as bv64)
-        else if (size == 2) then
-            (mem[off] as bv64) | (((mem[off+1] as bv64) & 0xff) << 8)
-        else if (size == 4) then
-            (mem[off] as bv64)                     | (((mem[off+1] as bv64) & 0xff) << 8)   |
-            (((mem[off+2] as bv64) & 0xff) << 16)  | (((mem[off+3] as bv64) & 0xff) << 24)
-        else
-            (mem[off] as bv64)                     | (((mem[off+1] as bv64) & 0xff) << 8)   |
-            (((mem[off+2] as bv64) & 0xff) << 16)  | (((mem[off+3] as bv64) & 0xff) << 24)  |
-            (((mem[off+4] as bv64) & 0xff) << 32)  | (((mem[off+5] as bv64) & 0xff) << 40)  |
-            (((mem[off+6] as bv64) & 0xff) << 48)  | (((mem[off+7] as bv64) & 0xff) << 56)
-    }      
+        var (rid, memid, cur_off) := get_ptr_info(addr_tv, ioff);
 
+        var data := s.mems[rid][memid].data;
+        var mem_type := s.mems[rid][memid].mem_type;
+        var slot_1st_tv := data[cur_off].etypev;
 
+        assert {:split_here} true;
+        var same_slot := ptr_slots_same_type_perm(data, cur_off, size);
 
-/**
-ghost function loadNbytesStack(mem: array<bv8>, memLen: int64, off: int64, idx:int64, size: int64) :bv64
-    reads mem
-    requires mem.Length == 512
-    requires size == 1 || size == 2 || size == 4 || size == 8
-    requires 0<= idx <= size
-    requires 0 <=  off+idx <= off+size <= 512
-    decreases size-idx
-    ensures size == 4 ==> loadNbytesStack(mem, off, idx, size) & 0xFFFF_FFFF_0000_0000 == 0x0
-    ensures size == 2 ==> loadNbytesStack(mem, off, idx, size) & 0xFFFF_FFFF_FFFF_0000 == 0x0
-    ensures size == 1 ==> loadNbytesStack(mem, off, idx, size) & 0xFFFF_FFFF_FFFF_FF00 == 0x0
-    {
-        if idx == size then (0x0 as bv64)
-        else ((mem[off+idx] as bv64) << ((idx * 8) as bv6)) | loadNbytesStack(mem, off, idx+1, size)
-    }
- */
+        assert {:split_here} true;
+        var nsize_val1 := read_n_byte_data(data, cur_off, size, sign_ext);
+        var ext_val1 := if sign_ext
+            then signext_byte_nto8(nsize_val1, size)
+            else nsize_val1;
 
-////////////////////////////////
-
-predicate ScalarTypes(regType: REGTYPE)
-    {
-        regType == SCALAR || regType == STACK_DYNPTR || regType == STACK_ITER
-    }
-
-predicate Ptr_or_NULL(regType: REGTYPE)
-    {
-        regType != UNINT && regType != SCALAR && regType != STACK_DYNPTR && regType != STACK_ITER
-    }
-
-predicate NonNULLPtr(regType: REGTYPE)
-    {
-        // exclude UNINT either
-        Ptr_or_NULL(regType) && regType != NULL
-    }
-
-predicate isMapPtr(regType: REGTYPE)
-    {
-        regType == MAP_PTR || regType == PTR_TO_MAP_KEY || regType == PTR_TO_MAP_VALUE
-    }
-
-predicate isPktPtr(regType: REGTYPE)
-    {
-        regType == PTR_TO_PACKET_META || regType == PTR_TO_PACKET || regType == PTR_TO_PACKET_END
-    }
-
-
-function MaskUpBySize(num: bv64, size: int64) :bv64
-    requires size == 1 || size == 2 || size == 4 || size == 8
-    {
-        if size == 1 then num & 0x0000_0000_0000_00FF
-        else if size == 2 then num & 0x0000_0000_0000_FFFF
-        else if size == 4 then num & 0x0000_0000_FFFF_FFFF
-        else num // size == 8
-    }
-
-
-////////////////////////////////// SOCKET Pointers ////////////////////////
-
-ghost predicate validate_sock_common_access(off: int64, size: int64)
-    {
-        // Cannot access fileds [type, protocol, mark, priority]
-        (off < 8 || off >= 24)
-        &&
-        validate_sock_access(off, size)
-    }
-
-// bpf_sock_is_valid_access, struct bpf_sock
-ghost predicate validate_sock_access(off: int64, size: int64)
-    {
-        (0 <= off < off + size < 80) &&
-        (
-            // 0 4 bound_dev_if
-            exact_4_read(off, size, 0, READ)
-            ||
-            
-            // 4 4 family
-            narrow_4_read_from_off(off, size, 4, READ)
-            ||
-            
-            // 8 4 type
-            narrow_4_read_from_off(off, size, 8, READ)
-            ||
-            
-            // 12 4 protocol
-            narrow_4_read_from_off(off, size, 12, READ)
-            ||
-            
-            // 16 4 mark
-            exact_4_read(off, size, 16, READ)
-            ||
-            
-            // 20 4 priority
-            exact_4_read(off, size, 20, READ)
-            ||
-            
-            // 24 4 src_ip4
-            narrow_4_read(off, size, 24, READ)
-            ||
-
-            // 28 16 src_ip6[4]
-            (
-                (28 <= off < off + size < 44) &&
-                (size == 1 || size == 2 || size == 4)
+        assert {:split_here} true;
+        match slot_1st_tv {
+                
+            case Scalar(k, _) => (
+                assert {:split_here} true;
+                if addr_tv.r == PTR_TO_CTX && size == W && k == SpecialPtr then
+                    if cur_off == 0 || cur_off == 76 then
+                        assert packet_mems_exist(s);
+                        PtrType(PTR_TO_PACKET_DATA, 0, 0)
+                    else if cur_off == 4 || cur_off == 80 then
+                        assert packet_mems_exist(s);
+                        PtrType(PTR_TO_PACKET_END, 0, 0)
+                    else if cur_off == 8 || cur_off == 140 then
+                        assert packet_mems_exist(s);
+                        PtrType(PTR_TO_PACKET_META, 0, 0)
+                    else
+                        Scalar(Normal, ext_val1)
+                else
+                    var new_kind := if same_slot then k else Normal;
+                    Scalar(new_kind, ext_val1)
             )
-            ||
 
-            // 44 4 src_port
-            narrow_4_read_from_off(off, size, 44, READ)
-            ||
+            case PtrType(_, _, _) | PtrOrNullType(_, _, _) => (
+                    
+                var alg_off := cur_off - (cur_off % 8);
+                assert {:split_here} (
+                    0 <= alg_off < alg_off + 8 <= |data|
+                    &&
+                    ptr_slots_same_type_perm(data, cur_off, size)
+                    &&
+                    forall i | alg_off <= i < alg_off + 8
+                    ::
+                    ptr_or_ptrornull(data[i].etypev)
+                ) by {
+                    valid_ptr_slots_implies_8_bytes(s, addr_tv, ioff, size);
+                }
+                    
+                assert {:split_here} true;
 
-            // 48 2 dst_port
-            // 50 2 padding
-            (off == 48 && (size == 2 || size == 4))
-            ||
+                if !same_slot
+                then (
+                    assert {:split_here} true;
+                    assert false;
+                    slot_1st_tv // Unreachable
+                    
+                )
+                else (
 
-            // 52 4 dst_ip4
-            narrow_4_read(off, size, 52, READ)
-            ||
+                    assert {:split_here} true;
+                    var val_8b  := read_8_byte_data(data, alg_off);
 
-            // 56 16 dst_ip6[4]
-            (
-                (56 <= off < off + size < 72) &&
-                (size == 1 || size == 2 || size == 4)
+                    assert {:split_here} true;
+                    if size == DW then (
+                        if is_ptr(slot_1st_tv)
+                        then PtrType(slot_1st_tv.r, slot_1st_tv.memid, val_8b)
+                        else PtrOrNullType(
+                            slot_1st_tv.r, slot_1st_tv.memid, val_8b
+                        )
+                        
+                    ) else (
+
+                        var rid      := r2id(slot_1st_tv.r);
+                        var memid    := slot_1st_tv.memid;
+
+                        assert {:split_here} true;
+                        // Pointer absolute value: base + offset
+                        var ptr_val := s.mems[rid][memid].base + val_8b;
+                        // Read N size and do sign-extension
+                        var nsize_val := low_nsize(ptr_val, size);   
+                        var ext_val2 := 
+                            if sign_ext
+                            then signext_byte_nto8(nsize_val, size)
+                            else nsize_val;
+
+                        // Final result depens on PtrType or PtrOrNullType
+                        assert {:split_here} true;
+                        if is_ptr(slot_1st_tv) then (
+                            Scalar(Normal, ext_val2)
+                        ) else (
+                            var unknown: bool :| true;
+                            // arith value of null_or_ptr: ptr arith or 0
+                            if unknown
+                            then Scalar(Normal, ext_val2)
+                            else Scalar(Normal, 0)
+                        )
+                    )
+                )
             )
-            ||
 
-            // 72 4 state
-            narrow_4_read_from_off(off, size, 72, READ)   ||
+            case Uninit => (
+                assert {:split_here} true;
+                assert false;
+                slot_1st_tv // Unreachable
+            )
+        }
+    }
+    
+    lemma valid_ptr_slots_implies_8_bytes(
+        s: State, addr_tv: ETYPEV, ioff: s16, size: SIZE
+    )
+    requires is_ptr(addr_tv) && valid_etypev_if_ptr(s, addr_tv)
+    requires access_mem_slots_valid(s, addr_tv, ioff, size)
+    requires var (rid, memid, cur_off) := get_ptr_info(addr_tv, ioff);
+             var slot_1st_tv := s.mems[rid][memid].data[cur_off].etypev;
+             ptr_or_ptrornull(slot_1st_tv)
+    //
+    ensures var (rid, memid, cur_off) := get_ptr_info(addr_tv, ioff);
+            var data := s.mems[rid][memid].data;
+            (
+                exists i | cur_off <= i < cur_off + size_to_nat(size)
+                ::
+                ptr_or_ptrornull(data[i].etypev)
+            )
+    //
+    ensures var (rid, memid, cur_off) := get_ptr_info(addr_tv, ioff);
+            var data := s.mems[rid][memid].data;
+            var alg_off := cur_off -(cur_off % 8);
+            0 <= alg_off < alg_off + 8 <= |data|
+            &&
+            (forall i | alg_off <= i < alg_off + 8
+            ::
+            ptr_or_ptrornull(data[i].etypev)
+            )
+            &&
+            ptr_slots_same_type_perm(data, cur_off, DW)
+    {}
 
-            // 76 4 rx_queue_mapping
-            narrow_4_read_from_off(off, size, 164, READ)
+    ghost function {:timeLimit 10} reg_to_8byte_data(
+        s: State, reg_tv: ETYPEV
+    ) : (res: seq<ETYPEV>)
+    //
+    requires valid_etypev_if_ptr(s, reg_tv)
+    requires reg_tv != Uninit
+    ensures |res| == 8
+    ensures valid_ptr_etypvs(s, res, DW)
+    {
+        match reg_tv {
+            case Scalar(k, v) =>
+                [
+                    Scalar(k, get_nth_byte(v, 0)),
+                    Scalar(k, get_nth_byte(v, 1)),
+                    Scalar(k, get_nth_byte(v, 2)),
+                    Scalar(k, get_nth_byte(v, 3)),
+                    Scalar(k, get_nth_byte(v, 4)),
+                    Scalar(k, get_nth_byte(v, 5)),
+                    Scalar(k, get_nth_byte(v, 6)),
+                    Scalar(k, get_nth_byte(v, 7))
+                ]
+
+            case PtrType(r, memid, off) =>
+                [
+                    PtrType(r, memid, get_nth_byte(off, 0)),
+                    PtrType(r, memid, get_nth_byte(off, 1)),
+                    PtrType(r, memid, get_nth_byte(off, 2)),
+                    PtrType(r, memid, get_nth_byte(off, 3)),
+                    PtrType(r, memid, get_nth_byte(off, 4)),
+                    PtrType(r, memid, get_nth_byte(off, 5)),
+                    PtrType(r, memid, get_nth_byte(off, 6)),
+                    PtrType(r, memid, get_nth_byte(off, 7))
+                ]
+
+            case PtrOrNullType(r, memid, off) =>
+                [
+                    PtrOrNullType(r, memid, get_nth_byte(off, 0)),
+                    PtrOrNullType(r, memid, get_nth_byte(off, 1)),
+                    PtrOrNullType(r, memid, get_nth_byte(off, 2)),
+                    PtrOrNullType(r, memid, get_nth_byte(off, 3)),
+                    PtrOrNullType(r, memid, get_nth_byte(off, 4)),
+                    PtrOrNullType(r, memid, get_nth_byte(off, 5)),
+                    PtrOrNullType(r, memid, get_nth_byte(off, 6)),
+                    PtrOrNullType(r, memid, get_nth_byte(off, 7))
+                ]
+
+            case _ => (
+                assert false;
+                []
+            )
+
+        }
+    }
+
+    /* off points to the byte offset of value in tv */
+    ghost function {:timeLimit 10} scalar_etypev_to_seq(
+        tv: ETYPEV, len: nat, cur_off: nat
+    ) :(res: seq<ETYPEV>)
+    //
+    requires is_scalar(tv)
+    requires 0 <= cur_off <= cur_off + len <= 8
+    ensures |res| == len
+    ensures forall i | 0 <= i < |res| :: is_scalar(res[i])
+    {
+        match len {
+            case 0 => []
+            case 1 => [Scalar(tv.kind, get_nth_byte(tv.val, cur_off+0))]
+            case 2 => [
+                Scalar(tv.kind, get_nth_byte(tv.val, cur_off + 0)),
+                Scalar(tv.kind, get_nth_byte(tv.val, cur_off + 1))
+            ]
+            case 3 => [
+                Scalar(tv.kind, get_nth_byte(tv.val, cur_off + 0)),
+                Scalar(tv.kind, get_nth_byte(tv.val, cur_off + 1)),
+                Scalar(tv.kind, get_nth_byte(tv.val, cur_off + 2))
+            ]
+            case 4 => [
+                Scalar(tv.kind, get_nth_byte(tv.val, cur_off + 0)),
+                Scalar(tv.kind, get_nth_byte(tv.val, cur_off + 1)),
+                Scalar(tv.kind, get_nth_byte(tv.val, cur_off + 2)),
+                Scalar(tv.kind, get_nth_byte(tv.val, cur_off + 3))
+            ]
+            case 5 => [
+                Scalar(tv.kind, get_nth_byte(tv.val, cur_off + 0)),
+                Scalar(tv.kind, get_nth_byte(tv.val, cur_off + 1)),
+                Scalar(tv.kind, get_nth_byte(tv.val, cur_off + 2)),
+                Scalar(tv.kind, get_nth_byte(tv.val, cur_off + 3)),
+                Scalar(tv.kind, get_nth_byte(tv.val, cur_off + 4))
+            ]
+            case 6 => [
+                Scalar(tv.kind, get_nth_byte(tv.val, cur_off + 0)),
+                Scalar(tv.kind, get_nth_byte(tv.val, cur_off + 1)),
+                Scalar(tv.kind, get_nth_byte(tv.val, cur_off + 2)),
+                Scalar(tv.kind, get_nth_byte(tv.val, cur_off + 3)),
+                Scalar(tv.kind, get_nth_byte(tv.val, cur_off + 4)),
+                Scalar(tv.kind, get_nth_byte(tv.val, cur_off + 5))
+            ]
+            case 7 => [
+                Scalar(tv.kind, get_nth_byte(tv.val, cur_off + 0)),
+                Scalar(tv.kind, get_nth_byte(tv.val, cur_off + 1)),
+                Scalar(tv.kind, get_nth_byte(tv.val, cur_off + 2)),
+                Scalar(tv.kind, get_nth_byte(tv.val, cur_off + 3)),
+                Scalar(tv.kind, get_nth_byte(tv.val, cur_off + 4)),
+                Scalar(tv.kind, get_nth_byte(tv.val, cur_off + 5)),
+                Scalar(tv.kind, get_nth_byte(tv.val, cur_off + 6))
+            ]
+            case 8 => [
+                Scalar(tv.kind, get_nth_byte(tv.val, cur_off + 0)),
+                Scalar(tv.kind, get_nth_byte(tv.val, cur_off + 1)),
+                Scalar(tv.kind, get_nth_byte(tv.val, cur_off + 2)),
+                Scalar(tv.kind, get_nth_byte(tv.val, cur_off + 3)),
+                Scalar(tv.kind, get_nth_byte(tv.val, cur_off + 4)),
+                Scalar(tv.kind, get_nth_byte(tv.val, cur_off + 5)),
+                Scalar(tv.kind, get_nth_byte(tv.val, cur_off + 6)),
+                Scalar(tv.kind, get_nth_byte(tv.val, cur_off + 7))
+            ]
+            case _ => (
+                assert false;
+                []
+            )
+        }
+    }
+
+    ghost function update_mem_slots(
+        s: State, mem_type : MEMTYPE, data: seq<MemSlot>,
+        cur_off: int, size: SIZE, new_tvs: seq<ETYPEV>
+    ) : (res: seq<MemSlot>)
+    //
+    requires size_to_nat(size) == |new_tvs|
+    requires 0 <= cur_off < cur_off + size_to_nat(size) <= |data|
+    requires valid_ptr_etypvs(s, new_tvs, size)
+    // Complementary conditions to `valid_ptr_etypvs`
+    requires mem_type == RAW ==> (
+                forall i | 0 <= i < size_to_nat(size)
+                :: !ptr_or_ptrornull(new_tvs[i])
+             )
+    //
+    requires access_slots_valid(s, mem_type, data, cur_off, size)
+    //
+    // All slots have the same RDWR perm
+    // Otherwise, storing a pointer could lead to different byte perms
+    requires forall i | cur_off <= i < cur_off + size_to_nat(size)
+             :: data[i].field_perm == RDWR
+    // If overwrites pointer slots, it must be complete overwrite
+    requires ptr_or_ptrornull(data[cur_off].etypev) ==> size == DW
+    //
+    ensures |data| == |res|
+    // Modified slots keeps previous perm and field size
+    ensures forall i | 0 <= i < size_to_nat(size)
+            ::
+            res[cur_off + i].etypev == new_tvs[i]
+            &&
+            res[cur_off + i].field_perm == data[cur_off + i].field_perm
+            &&
+            res[cur_off + i].field_size == data[cur_off + i].field_size
+            // &&
+            // res[cur_off + i].etypev != Uninit
+    ensures forall i | 0 <= cur_off <= i < cur_off +size_to_nat(size)
+            :: res[i].etypev != Uninit
+    // Unmodified slots keep unchanged
+    ensures forall j |
+            0 <= j < cur_off || cur_off + size_to_nat(size) <= j < |data|
+            ::
+            res[j] == data[j]
+    //
+    ensures access_slots_valid(s, mem_type, res, cur_off, size)
+    {
+        match size {
+            
+            case B =>
+                data[cur_off + 0 := data[cur_off + 0].(etypev := new_tvs[0])]
+            
+            case HW =>
+                data
+                [cur_off + 0 := data[cur_off + 0].(etypev := new_tvs[0])]
+                [cur_off + 1 := data[cur_off + 1].(etypev := new_tvs[1])]
+            
+            case W =>
+                data
+                [cur_off + 0 := data[cur_off + 0].(etypev := new_tvs[0])]
+                [cur_off + 1 := data[cur_off + 1].(etypev := new_tvs[1])]
+                [cur_off + 2 := data[cur_off + 2].(etypev := new_tvs[2])]
+                [cur_off + 3 := data[cur_off + 3].(etypev := new_tvs[3])]
+            
+            case DW =>
+                data
+                [cur_off + 0 := data[cur_off + 0].(etypev := new_tvs[0])]
+                [cur_off + 1 := data[cur_off + 1].(etypev := new_tvs[1])]
+                [cur_off + 2 := data[cur_off + 2].(etypev := new_tvs[2])]
+                [cur_off + 3 := data[cur_off + 3].(etypev := new_tvs[3])]
+                [cur_off + 4 := data[cur_off + 4].(etypev := new_tvs[4])]
+                [cur_off + 5 := data[cur_off + 5].(etypev := new_tvs[5])]
+                [cur_off + 6 := data[cur_off + 6].(etypev := new_tvs[6])]
+                [cur_off + 7 := data[cur_off + 7].(etypev := new_tvs[7])]
+        }
+    }
+
+    ghost function update_a_mem_in_state(
+        s: State, addr_tv: ETYPEV, new_data: seq<MemSlot>
+    ) : (res: State)
+    requires is_ptr(addr_tv) && valid_etypev_if_ptr(s, addr_tv)
+    {
+        var (rid, memid, _) := get_ptr_info(addr_tv, 0);
+        s.(mems := (
+                s.mems[rid :=
+                    s.mems[rid][memid := 
+                        s.mems[rid][memid].(data := new_data)
+                    ]
+                ]
+            )
         )
-        //
     }
 
-// bpf_tcp_sock_is_valid_access, struct bpf_tcp_sock
-ghost predicate validate_tcp_sock_access(off: int64, size: int64)
+    ghost predicate same_mem_region(s: State, dst: REG, src: REG)
     {
-        (if off == 80 || off == 88 then size == 8 else size == 4)       &&
-        (0 <= off < off + size < 112) // sizeof(struct bpf_tcp_sock)
+        var dst_tv := get_reg_typeval(s, dst);
+        var src_tv := get_reg_typeval(s, src);
+
+        is_ptr(dst_tv) && is_ptr(src_tv)
+        &&
+        dst_tv == src_tv
+        &&
+        dst_tv.memid == src_tv.memid
     }
 
-// bpf_xdp_sock_is_valid_access, struct bpf_xdp_sock
-ghost predicate validate_xdp_sock_access(off: int64, size: int64)
+    function {:axiom} sim_concur_mem_val(
+        s: State, addr_reg: REG, size: SIZE
+    ) : (res: ETYPEV)
+    requires mem_inv(s)
+    requires is_ptr(get_reg_typeval(s, addr_reg))
+    ensures res != Uninit
+    ensures size != DW ==> is_scalar(res)
+    ensures var (rid, memid, _) :=
+            get_ptr_info(get_reg_typeval(s, addr_reg), 0);
+            s.mems[rid][memid].mem_type == RAW ==>
+                is_scalar(res)
+    ensures valid_etypev_if_ptr(s, res)
+
+
+    lemma {:axiom} axiom_on_concur(
+        s1: State, s2: State, addr_reg: REG, size: SIZE
+    )
+    requires mem_inv(s1)
+    requires mem_inv(s2)
+    requires is_ptr(get_reg_typeval(s1, addr_reg))
+    requires is_ptr(get_reg_typeval(s2, addr_reg))
+    requires s1.rand == s2.rand
+    ensures sim_concur_mem_val(s1, addr_reg, size) ==
+            sim_concur_mem_val(s2, addr_reg, size)
+
+
+    ghost function get_addr(s: State, reg: REG) : (res: bv64)
+    requires var regtv := get_reg_typeval(s, reg);
+             ptr_or_ptrornull(regtv) && valid_etypev_if_ptr(s, regtv)
     {
-        off == 0 && size == 4
-        /*
-            struct bpf_xdp_sock {
-                __u32 queue_id;
-            };
-            */
+        var regtv := get_reg_typeval(s, reg);
+
+        var (r, memid, off) := (regtv.r, regtv.memid, regtv.off);
+        var tid := r2id(regtv.r);
+        
+        s.mems[tid][memid].base + off
     }
 
-ghost predicate unknown_bool()
-
-method AnyBv64() returns (x: bv64)
-{
-  x :| true;  // Non-deterministically assign any value to x
-}
-
-method AnyInt64() returns (x: int64)
-{
-  x :| true;  // Non-deterministically assign any value to x
-}
-
-method AnyRegtype() returns (x: REGTYPE)
-{
-  x :| true;  // Non-deterministically assign any value to x
-}
-
-method AnyBv8() returns (x: bv8)
-{
-  x :| true;  // Non-deterministically assign any value to x
-}
+    ghost function get_base_addr(s: State, reg: REG) : (res: bv64)
+    requires var regtv := get_reg_typeval(s, reg);
+             ptr_or_ptrornull(regtv) && valid_etypev_if_ptr(s, regtv)
+    {
+        var regtv := get_reg_typeval(s, reg);
+        var tid := r2id(regtv.r);
+        
+        s.mems[tid][regtv.memid].base
+    }
 
 
-ghost predicate unknownBv64(x: bv64) {
-    0x0000_0000_0000_0000 <= x <= 0xFFFF_FFFF_FFFF_FFFF
-}
+    // TODO: enusres are not verified
+    function {:axiom} new_base_addr(s: State, t: ETYPEV, size: bv64) : (res: bv64)
+    requires ptr_or_ptrornull(t)
+    // The memory region does not exist in the s.mems
+    requires var (r, memid, off) := (t.r, t.memid, t.off);
+             var rid := r2id(t.r);
+             (rid >= |s.mems| || (0 <= rid < |s.mems| && memid >= |s.mems[rid]|))
+    //
+    requires mem_inv(s)
+    //
+    requires 0 <= r2id(PTR_TO_PACKET_META) < |s.mems|
+    requires |s.mems[r2id(PTR_TO_PACKET_META)]| == 1
+    requires 0 <= r2id(PTR_TO_PACKET_DATA) < |s.mems|
+    requires |s.mems[r2id(PTR_TO_PACKET_DATA)]| == 1
+    //
+    ensures res != 0
+    ensures (
+                forall i,j | 0 <= i < |s.mems| && 0 <= j < |s.mems[i]| :: (
+                    var base1 := s.mems[i][j].base;
+                    var size1 := (|s.mems[i][j].data| as bv64);
+                    //
+                    // Non-overlapped memory regions
+                    base1 != res
+                    &&
+                    (base1 + size1 <= res  ||  res + size <= base1)
+                )
+            )
+            &&
+            (
+                t.r == PTR_TO_PACKET_DATA ==> (
+                    var base_meta := s.mems[r2id(PTR_TO_PACKET_META)][0].base;
+                    var size_meta := (|s.mems[r2id(PTR_TO_PACKET_META)][0].data| as bv64);
+                    base_meta + size_meta == res
+                )
+            )
+            &&
+            (
+                t.r == PTR_TO_PACKET_END ==> (
+                    var base_data := s.mems[r2id(PTR_TO_PACKET_DATA)][0].base;
+                    var size_data := (|s.mems[r2id(PTR_TO_PACKET_DATA)][0].data| as bv64);
+                    base_data + size_data == res
+                    &&
+                    size == 0
+                )
+            )
+    
 
-ghost predicate unknownBv32(x: bv64) {
-    0x0000_0000_0000_0000 <= x <= 0x0000_0000_FFFF_FFFF
-}
+    lemma diff_r_diff_id(r1: MemRegion, r2: MemRegion)
+    requires r1 != r2
+    ensures r2id(r1) != r2id(r2)
+    {}
 
-ghost predicate unknownBv(x: bv64, size:int) {
-    if size == 1 then 0 <= x <= 0xFF
-    else if size == 2 then 0 <= x <= 0xFF_FF
-    else if size == 4  then 0 <= x <= 0xFF_FF_FF_FF
-    else if size == 8 then 0 <= x <= 0xFFFF_FFFF_FFFF_FFFF
-    else false
+    /*
+    lemma diff_base(s: State, reg1: REG, reg2: REG)
+    requires (
+        var regtv1 := get_reg_typeval(s, reg1);
+        var regtv2 := get_reg_typeval(s, reg2);
+        
+        ptr_or_ptrornull(regtv1)
+        &&
+        ptr_or_ptrornull(regtv2)
+        &&
+        (regtv1.r != regtv2.r || regtv1.memid != regtv2.memid)
+    )
+    requires mem_inv(s)
+    ensures get_base_addr(s, reg1) != get_base_addr(s, reg2)
+    {
+        var regtv1 := get_reg_typeval(s, reg1);
+        var regtv2 := get_reg_typeval(s, reg2);
+
+        assert regtv1.r != regtv2.r || regtv1.memid != regtv2.memid;
+        
+        assert {:split_here} r2id(regtv1.r) != r2id(regtv2.r) || regtv1.memid != regtv2.memid by {
+            if regtv1.r != regtv2.r {
+                assert {:split_here} r2id(regtv1.r) != r2id(regtv2.r);
+            }
+            else {
+                assert {:split_here} regtv1.memid != regtv2.memid;
+            }
+        }
+        
+        assert {:split_here} (r2id(regtv1.r), regtv1.memid) != (r2id(regtv2.r), regtv2.memid);
+        
+        assert {:split_here} s.mems[r2id(regtv1.r)][regtv1.memid].base != s.mems[r2id(regtv2.r)][regtv2.memid].base;
+        
+        var b1 := get_base_addr(s, reg1);
+        var b2 := get_base_addr(s, reg2);
+
+        assert {:split_here} s.mems[r2id(regtv1.r)][regtv1.memid].base == b1;
+        assert {:split_here} s.mems[r2id(regtv2.r)][regtv2.memid].base == b2;
+
+        assert {:split_here} get_base_addr(s, reg1) != get_base_addr(s, reg2) by {
+            assert b1 != b2;
+        }
+    }
+
+    lemma diff_base_2(s: State, r1: nat, memid1: nat, r2: nat, memid2: nat)
+    requires mem_inv(s)
+    requires r1 != r2 || memid1 != memid2
+    requires 0 <= r1 < |s.mems|
+    requires 0 <= r2 < |s.mems|
+    requires 0 <= memid1 < |s.mems[r1]|
+    requires 0 <= memid2 < |s.mems[r2]|
+    ensures s.mems[r1][memid1].base != s.mems[r2][memid2].base
+    {}
+    */
+
+    lemma same_base(s: State, reg1: REG, reg2: REG)
+    requires (
+        var regtv1 := get_reg_typeval(s, reg1);
+        var regtv2 := get_reg_typeval(s, reg2);
+        
+        ptr_or_ptrornull(regtv1)
+        &&
+        ptr_or_ptrornull(regtv2)
+        &&
+        (regtv1.r == regtv2.r && regtv1.memid == regtv2.memid)
+    )
+    requires mem_inv(s)
+    ensures get_base_addr(s, reg1) == get_base_addr(s, reg2)
+    {}
+
+
+    ghost predicate packet_mems_exist(s: State)
+    {
+        0 <= r2id(PTR_TO_PACKET_META) < |s.mems|
+        &&
+        0 < |s.mems[r2id(PTR_TO_PACKET_META)]|
+        &&
+        0 <= r2id(PTR_TO_PACKET_DATA) < |s.mems|
+        &&
+        0 < |s.mems[r2id(PTR_TO_PACKET_DATA)]|
+        &&
+        0 <= r2id(PTR_TO_PACKET_END) < |s.mems|
+        &&
+        0 < |s.mems[r2id(PTR_TO_PACKET_END)]|
+    }
+
+    ghost predicate mem_inv(s: State)
+    {
+        (
+            // Memory region size
+            forall i, j | 0 <= i < |s.mems| && 0 <= j < |s.mems[i]| ::
+                if i == r2id(PTR_TO_PACKET_END)
+                then 0 == |s.mems[i][j].data|
+                else 0 <= |s.mems[i][j].data| < 0x8000_0000_0000_0000
+        )
+        &&
+        packet_mems_exist(s)
+        &&
+        (
+            // Valid pointer reg
+            forall reg :: valid_etypev_if_ptr(s, get_reg_typeval(s, reg))
+        )
+    }
+
+    ghost predicate access_mem_slots_valid(
+        s: State, addr_tv: ETYPEV, ioff: s16, size: SIZE
+    )
+    requires is_ptr(addr_tv)
+    requires valid_etypev_if_ptr(s, addr_tv)
+    {
+        var (rid, memid, cur_off) := get_ptr_info(addr_tv, ioff);
+
+        var mem := s.mems[rid][memid];
+
+        var mem_type := mem.mem_type;
+        var data := mem.data;
+
+        access_slots_valid(s, mem_type, data, cur_off, size)
+    }
+
+    ghost predicate access_slots_valid(
+        s: State, mem_type: MEMTYPE,
+        data: seq<MemSlot>, cur_off: int, size: SIZE
+    )
+    {
+        0 <= cur_off < cur_off + size_to_nat(size) <= |data|
+        &&
+        // RAW memories are all Scalar(_, _)
+        if mem_type == RAW then (
+            (s.cfg.strict_alignment ==> cur_off % size_to_nat(size) == 0)
+            &&
+            (
+                forall i| cur_off <= i < cur_off + size_to_nat(size) <= |data|
+                ::
+                is_scalar(data[i].etypev)
+            )
+        )
+        // STRUCT:  scalars and pointers
+        // GENERAL: uninit, scalars, and pointers
+        else (
+            (cur_off % size_to_nat(size) == 0)
+            &&
+            (
+                var alg_off := cur_off - (cur_off % 8);
+                if (
+                    exists i | 0 <= alg_off <= i < alg_off + 8
+                    ::
+                    i < |data|
+                    &&
+                    ptr_or_ptrornull(data[i].etypev)
+                ) then (
+                    (cur_off == alg_off)
+                    &&
+                    0 <= alg_off < alg_off + 8 <= |data|
+                    &&
+                    // ptr slots have the same type and perm
+                    ptr_slots_same_type_perm(data, alg_off, DW)
+                    &&
+                    // rid and memid in the slots are valid
+                    var slot_tv := data[cur_off].etypev;
+                    valid_etypev_if_ptr(s, slot_tv)
+                ) else (
+                    forall i |
+                    cur_off <= i < cur_off + size_to_nat(size) <= |data|
+                    ::
+                    (
+                        (mem_type == STRUCT ==> is_scalar(data[i].etypev))
+                        &&
+                        (mem_type == GENERAL ==>
+                            !ptr_or_ptrornull(data[i].etypev))
+                    )
+                )
+            )
+        )
+    }
+
+    predicate ptr_slots_same_type_perm(
+        data: seq<MemSlot>, cur_off: int, size: SIZE
+    )
+    requires 0 <= cur_off < cur_off + size_to_nat(size) <= |data|
+    {
+        var sizen := size_to_nat(size);
+
+        match data[cur_off].etypev {
+        
+            case PtrType     (r0, id0, _) =>
+                forall i | cur_off < i < cur_off + sizen ::
+                    match data[i].etypev {
+                        case PtrType     (r, id, _) =>
+                            r == r0 && id == id0
+                            &&
+                            data[i].field_perm == data[cur_off].field_perm
+                        case _  => false
+                    }
+
+            case PtrOrNullType(r0, id0, _) =>
+                forall i | cur_off < i < cur_off + sizen ::
+                    match data[i].etypev {
+                        case PtrOrNullType(r, id, _) =>
+                            r == r0 && id == id0
+                            &&
+                            data[i].field_perm == data[cur_off].field_perm
+                        case _  => false
+                    }
+            
+            case _ => false
+        }
+    }
+    
+    predicate ptr_slots_same_type(tvs: seq<ETYPEV>, cur_off: int, size: SIZE)
+    requires 0 <= cur_off < cur_off + size_to_nat(size) <= |tvs|
+    {
+        var sizen := size_to_nat(size);
+
+        match tvs[cur_off] {
+            case PtrType     (r0, id0, _) =>
+                forall i | cur_off < i < cur_off + sizen ::
+                    match tvs[i] {
+                        case PtrType     (r, id, _)  => (r == r0 && id == id0)
+                        case _                       => false
+                    }
+            
+            case PtrOrNullType(r0, id0, _) =>
+                forall i | cur_off < i < cur_off + sizen ::
+                    match tvs[i] {
+                        case PtrOrNullType(r, id, _) => (r == r0 && id == id0)
+                        case _                       => false
+                    }
+            
+            case _ => false
+        }
+    }
+
+    predicate valid_ptr_etypvs(s: State, tvs: seq<ETYPEV>, size: SIZE)
+    requires |tvs| == size_to_nat(size)
+    {
+        if size == DW && (
+            exists i | 0 <= i < size_to_nat(size)
+            ::
+            ptr_or_ptrornull(tvs[i])
+        ) then (
+            // ptr slots have the same type and perm
+            ptr_slots_same_type(tvs, 0, size)
+            &&
+            // rid and memid in the slots are valid
+            valid_etypev_if_ptr(s, tvs[0])
+        ) else (
+            forall i | 0 <= i < size_to_nat(size)
+            :: is_scalar(tvs[i])
+        )
+    }
+
+    predicate valid_etypev_if_ptr(s: State, regtv: ETYPEV) {
+        ptr_or_ptrornull(regtv) ==>
+            var (r, memid) := (regtv.r, regtv.memid);
+             var tid := r2id(regtv.r);
+             0 <= tid < |s.mems| && 0 <= memid < |s.mems[tid]|
+    }
 }
