build_syz.sh
@@ -1,0 +1,14 @@
+#!/bin/bash
+# Build translator first
+cd ~/veritas/shallow-embedding && make clean && make
+
+# Build syz-manager
+cd ~/veritas/syzkaller
+export PATH=$HOME/veritas/go-env/go/bin:$PATH
+REV="c1551704ab4760d0d65fb8e0d023606c8d69425b"
+DATE=$(date +%Y%m%d-%H%M%S)
+CGO_CXXFLAGS="-std=c++17 -I$HOME/veritas/shallow-embedding/src" \
+CGO_LDFLAGS="-L$HOME/veritas/shallow-embedding -lshallow-embedding -lstdc++ -lelf -lz -lzstd" \
+go build "-ldflags=-s -w -X github.com/google/syzkaller/prog.GitRevision=$REV -X github.com/google/syzkaller/prog.gitRevisionDate=$DATE" \
+  -o ./bin/syz-manager github.com/google/syzkaller/syz-manager
+echo "Done: $(ls -la bin/syz-manager)"
